CoqOfRust/links/M.v
@@ -230,6 +230,9 @@ Module Integer.
   Global Instance IsPrimitiveEq {kind : IntegerKind.t} : PrimitiveEq.Trait (t kind) := {
     PrimitiveEq.eqb x y := x.(value) =? y.(value);
   }.
+
+  Definition wrap_of_Z {kind : IntegerKind.t} (z : Z) : t kind :=
+    {| value := Integer.normalize_wrap kind z |}.
 End Integer.
 
 (** ** Integer kinds for better readability *)
@@ -1038,14 +1041,21 @@ Module LowM.
   Inductive t (R Output : Set) : Set :=
   | Pure (value : Output.t R Output)
   | CallPrimitive {A : Set} (primitive : Primitive.t A) (k : A -> t R Output)
-  | Call {A : Set} `{Link A} {e : M} (run : {{ e 🔽 A, A }}) (k : SuccessOrPanic.t A -> t R Output)
+  (* | Call {A : Set} `{Link A}
+      {e : M}
+      (run : {{ e 🔽 A, A }})
+      (k : SuccessOrPanic.t A -> t R Output) *)
+  | Call {A : Set}
+      (e : t A A)
+      (k : SuccessOrPanic.t A -> t R Output)
   | LetAlloc {A : Set} `{Link A}
       (e : t R A)
       (k : Output.t R (Ref.t Pointer.Kind.Raw A) -> t R Output)
   | Loop {A : Set} (body : t R A) (k : Output.t R A -> t R Output).
   Arguments Pure {_ _}.
   Arguments CallPrimitive {_ _ _}.
-  Arguments Call {_ _ _ _ _}.
+  (* Arguments Call {_ _ _ _ _}. *)
+  Arguments Call {_ _ _}.
   Arguments LetAlloc {_ _ _ _}.
   Arguments Loop {_ _ _}.
 End LowM.
@@ -1144,7 +1154,8 @@ Proof.
   }
   { (* CallClosure *)
     eapply (LowM.Call (A := Output')). {
-      exact run.
+      (* exact run. *)
+      exact (evaluate _ _ _ _ _ run).
     }
     intros output'; eapply evaluate.
     match goal with
